iris/ProofPipewrite.v
@@ -2208,13 +2208,16 @@ Section ProofPipewrite.
           assert (Hav14 : (14 <= trap_res true + (av - 14))%nat) by lia.
           (* killed() ONLY REPORTS THE FLAG (lane SELF-KILL, §4b'): the
              access this caller supplies is the identity. *)
-          iAssert (∀ (gn : gname) (klv : mword 32),
-                     SchedCtx.kill_row gn klv ==∗ SchedCtx.kill_row gn klv ∗ emp)%I
+          iAssert (∀ (pidr klr : mword 32),
+                     p_pid (proc_addr j) ↦₄{DfracOwn (1/4)} pidr -∗
+                     SchedCtx.kill_paid pidr klr -∗
+                     p_pid (proc_addr j) ↦₄{DfracOwn (1/4)} pidr ∗
+                     SchedCtx.kill_paid pidr klr ∗ emp)%I
             as "Hkacc".
-          { iIntros (gn klv) "H". iModIntro. iSplitL "H"; [ iExact "H" | done ]. }
+          { iIntros (pidr klr) "Hq Hr". iFrame "Hq Hr". }
           iApply (Killed.wp_killed_sconf γs j γlp L3 (trap_res true + (av - 14))%nat 1%nat true (proc_addr j) false
                     ({["pipe"]} ∪ lks)
-                    (fun (_ : gname) (_ : mword 32) => emp)%I
+                    (fun (_ : mword 32) => emp)%I
                     Ha0L3 Hj Hjlp Hlvl1 Hav14 ltac:(lkbelow)
                     with "Hkacc Hcg Hown Htext Hpc Hpinv").
           all: try lkbelow.
